\input ../SlidePreamble
\input ../preamble


\begin{document}

{\Huge

  \centerline{\bf TTIC 31230, Fundamentals of Deep Learning}
  \bigskip
  \centerline{David McAllester, Winter 2020}
  \vfill
  \centerline{\bf Noise Contrastive Estimation}
\vfill
\vfill

\slidetwo{Noise Contrastive Estimation}{Gutmann and Hyv\"{a}rinen, 2010}

{\color{red}
$$\Psi^* = \argmin_\Psi E_{(i,y_1,\ldots,y_{N}) \sim \tilde{p}_\Phi^{(N)}} \;- \ln P_\Psi(i|y_1,\ldots,y_{N})$$
\centerline{$p_\Phi$ is fixed ``noise''}
}

\vfill
Assume $p_\Phi$ is both samplable and computable --- we can sample from $p_\Phi$ and for any given $y$ we can compute $p_\Phi(y)$.

\vfill
Assume $P_\Psi(i|y_1,\ldots,y_{N}) = \softmax_i s_\Psi(y_i)$

\vfill
Assume $\Psi$ universal


\anaslide{Noise Contrastive Estimation}

$$\Psi^* = \argmin_\Psi E_{(i,y_1,\ldots,y_{N}) \sim \tilde{p}_\Phi^{(N)}} \;- \ln P_\Psi(i|y_1,\ldots,y_{N})$$
\centerline{$p_\Phi$ is fixed ``noise''}

\vfill
Theorem: {\color{red} $\popd(y) = \softmax_y\;\;\; s_{\Psi^*}(y) + \ln p_\Phi(y)$}

\vfill
We then have a computable score function (energy function) for the population.  We do not have the partition function $Z$.

\anaslide{Noise Contrastive Estimation}

$$\Psi^* = \argmin_\Psi E_{(i,y_1,\ldots,y_{N}) \sim \tilde{p}_\Phi^{(N)}} \;- \ln P_\Psi(i|y_1,\ldots,y_{N})$$
\centerline{$p_\Phi$ is fixed ``noise''}

\vfill
Lemma: {\color{red} $P_{\Psi^*}(i|y_1,\ldots,y_{N})  =  \softmax_i\;\; \ln \frac{\popd(y_i)}{p_\Phi(y_i)}$}

\slide{Lemma Proof}
{\huge
\begin{eqnarray*}
{\color{red} \tilde{p}_\Phi^{(N)}(i \;\mathrm{and}\;y_1,\ldots,y_{N})} & = & \frac{1}{N}\;\popd(y_i)\prod_{j \not = i}p_\Phi(y_j) \\
\\
& = & \alpha \frac{\popd(y_i)}{p_\Phi(y_i)},\;\;\;\alpha = \frac{1}{N} \prod_i p_\Phi(y_i) \\
\\
\\
{\color{red} \tilde{p}_\Phi^{(N)}(i\;|\;y_1,\ldots y_{N})} & = & \frac{\tilde{p}_\Phi^{(N)}(i\;\mbox{and} \; y_1,\ldots,y_{N})}{\sum_i \;\tilde{p}_\Phi^{(N)}(i \;\mbox{and}\; y_1,\ldots,y_{N})} \;=\;\frac{1}{Z} \;\frac{\popd(y_i)}{p_\Phi(y_i)} \\
\\
\\
& = & {\color{red} \softmax_i\; \left(\ln \frac{\popd(y_i)}{p_\Phi(y_i)}\right)}
\end{eqnarray*}
}

\slide{Theorem Proof}

$$\softmax_i s_{\Psi^*}(y_i) =  \softmax_i \ln \frac{\popd(y_i)}{p_\Phi(y_i)}$$

\vfill
is solved by

\vfill
$$s_{\Psi^*}(y) = \ln \frac{\popd(y)}{p_\Phi(y)} + \ln Z$$

\vfill
giving

$$\popd(y) = \frac{1}{Z} \exp(s_\Psi(y) + \ln p_\Phi(y))$$

\slide{END}

}
\end{document}


\slide{Another Theorem}

\begin{eqnarray*}
  && E_{(i,y_1,\dots,y_{N}) \sim \tilde{p}_\Phi^{(N)}}\;- \ln p^{(N)}_{\Psi^*}(i|y_1,\ldots,y_{N}) \\
  \\
  \\
  \\
  & \geq & \ln N - \frac{N-1}{N}(KL(\popd,p_\Phi) + KL(p_\Phi,\popd))
\end{eqnarray*}

\vfill
Note that the bound holds with equality for $p_\Phi = \popd$.

\vfill
This is analogous to the JSD expression for the optimal discriminator.
\slide{Proof Part A.}

{\huge
 \begin{eqnarray*}
    & & E_{(i,y_1,\ldots,y_{N}) \sim \tilde{p}_\Phi^{(N)}}\;\ln p_{\Psi^*}(i|y_1,\ldots,y_{N}) \\
    \\
    & = & E_{(i,y_1,\ldots,y_{N}) \sim \tilde{p}_\Phi^{(N)}}\;\ln \left(\softmax_i \;\ln \frac{\popd(y_i)}{p_\Phi(y_i)}\right)[i] \\
    \\
    & = & E_{(i,y_1,\ldots,y_{N}) \sim \tilde{p}_\Phi^{(N)}}\;\ln\frac{\popd(y_i)}{p_\Phi(y_i)} - \ln\left(\sum_j \frac{\popd(y_j)}{p_\Phi(y_j)} \right) \\
    \\
    & = & E_{(i,y_1,\ldots,y_{N}) \sim \tilde{p}_\Phi^{(N)}}\;\ln\frac{\popd(y_i)}{p_\Phi(y_i)} - \ln\left(\frac{1}{N}\sum_j \frac{\popd(y_j)}{p_\Phi(y_j)} \right) - \ln\;N
  \end{eqnarray*}
}

\slide{Proof Part B.}
{\huge
 \begin{eqnarray*}
    & & E_{(i,y_1,\ldots,y_{N}) \sim \tilde{p}_\Phi^{(N)}}\;\ln\frac{\popd(y_i)}{p_\Phi(y_i)} {\color{red} - \ln\left(\frac{1}{N}\sum_j \frac{\popd(y_j)}{p_\Phi(y_j)} \right)} - \ln\;N \\
    \\
    & {\color{red} \leq} & E_{(i,y_1,\ldots,y_{N}) \sim \tilde{p}_\Phi^{(N)}}\;\ln\frac{\popd(y_i)}{p_\Phi(y_i)} {\color{red} - \frac{1}{N} \sum_j \ln\frac{\popd(y_j)}{p_\Phi(y_j)}} - \ln\;N \\
    \\
    & = & E_{y \sim \popd} \ln \frac{\popd(y)}{p_\Phi(y)} -  E_{(i,y_1,\ldots,y_N) \sim \tilde{p}^{(N)}_\Phi} \frac{1}{N} \sum_j \ln\frac{\popd(y_j)}{p_\Phi(y_j)} - \ln N \\
    \\
    & = & \frac{N-1}{N}(KL(\popd,p_\Phi) + KL(p_\Phi,\popd)) - \ln\;N \\
  \end{eqnarray*}
}


\slide{Noise Descriminiative Estimation}

As in noise contrastive estimation we assume a noise distribution $p_\Phi$ that is both samplable and computable.

\vfill
For noise descriminative estimation, and for for $i \in \{-1,1\}$, we define a probability distribution over pairs
$\tuple{i,y}$ as in GANs.

\vfill

\begin{eqnarray*}
\tilde{p}_\Phi(i = 1) & = & 1/2 \\
\tilde{p}_\Phi(y|i=1) & =&  \popd(y) \\
\tilde{p}_\Phi(y|i=-1) & = & p_\Phi(y)
\end{eqnarray*}

\slide{Noise Discriminative Estimation}

\begin{eqnarray*}
  \Psi^* & = & \argmin_\Psi\;E_{\tuple{i,y} \sim \tilde{p}_\Phi}\;-\ln P_\Psi(i|y)
\end{eqnarray*}

\vfill
Assume $P_\Psi(i|y) = \softmax_i \;is_\Psi(y) = \frac{1}{1+e^{-2is_\Psi(y)}}$

\vfill
Assume $\Psi$ universal.

\anaslide{Noise Discriminative Estimation}

$$\Psi^* = \argmin_\Psi E_{(i,y) \sim \tilde{p}_\Phi} \;- \ln P_\Psi(i|y)$$

\vfill
Theorem: {\color{red} $\popd(y) = \softmax_y\;\;\; s_{\Psi^*}(y) + \ln p_\Phi(y)$}

\vfill
As with noise contrastive estimation, we have a computable score function (energy function) for the population.  We do not have the partition function $Z$.

\anaslide{Noise Discriminative Estimation}

$$\Psi^* = \argmin_\Psi E_{(i,y_1,\ldots,y_{N}) \sim \tilde{p}_\Phi^{(N)}} \;- \ln P_\Psi(i|y_1,\ldots,y_{N})$$

\vfill
Lemma: {\color{red} $P_{\Psi^*}(i|y)  =  \softmax_i\;is_{\Psi^*}(y)$}

\slide{Lemma Proof}
{\huge
\begin{eqnarray*}
{\color{red} \tilde{p}_\Phi^{(N)}(i \;\mathrm{and}\;y_1,\ldots,y_{N})} & = & \frac{1}{N}\;\popd(y_i)\prod_{j \not = i}p_\Phi(y_j) \\
\\
& = & \alpha \frac{\popd(y_i)}{p_\Phi(y_i)},\;\;\;\alpha = \frac{1}{N} \prod_i p_\Phi(y_i) \\
\\
\\
{\color{red} \tilde{p}_\Phi^{(N)}(i\;|\;y_1,\ldots y_{N})} & = & \frac{\tilde{p}_\Phi^{(N)}(i\;\mbox{and} \; y_1,\ldots,y_{N})}{\sum_i \;\tilde{p}_\Phi^{(N)}(i \;\mbox{and}\; y_1,\ldots,y_{N})} \;=\;\frac{1}{Z} \;\frac{\popd(y_i)}{p_\Phi(y_i)} \\
\\
\\
& = & {\color{red} \softmax_i\; \left(\ln \frac{\popd(y_i)}{p_\Phi(y_i)}\right)}
\end{eqnarray*}
}

\slide{Theorem Proof}

$$\softmax_i s_{\Psi^*}(y_i) =  \softmax_i \ln \frac{\popd(y_i)}{p_\Phi(y_i)}$$

\vfill
is solved by

\vfill
$$s_{\Psi^*}(y) = \ln \frac{\popd(y)}{p_\Phi(y)} + \ln Z$$

\vfill
giving

$$\popd(y) = \frac{1}{Z} \exp(s_\Psi(y) + \ln p_\Phi(y))$$
